11UnstructuredState/UnstructuredState.thy
@@ -25,13 +25,13 @@ fun unstr_lookup :: "(nat \<Rightarrow> nat) \<Rightarrow> nat \<Rightarrow> nat
 | "unstr_lookup h (Suc (Suc p)) (Suc x) = (if even p then unstr_lookup h (h (Suc p)) x else None)"
 
 inductive eval\<^sub>r :: "code\<^sub>b list \<Rightarrow> state\<^sub>r \<Rightarrow> state\<^sub>r \<Rightarrow> bool" (infix "\<tturnstile> _ \<leadsto>\<^sub>r" 50) where
-  ev\<^sub>r_lookup [simp]: "lookup \<C> p\<^sub>\<C> = Some (Lookup\<^sub>b x) \<Longrightarrow> unstr_lookup \<Delta> (s b\<^sub>s) x = Some y \<Longrightarrow>
+  ev\<^sub>r_lookup [simp]: "lookup \<C> p\<^sub>\<C> = Some (Lookup\<^sub>b x z w) \<Longrightarrow> unstr_lookup \<Delta> (s b\<^sub>s) x = Some y \<Longrightarrow>
     \<C> \<tturnstile> S\<^sub>r h b\<^sub>h \<Delta> b\<^sub>\<Delta> \<V> b\<^sub>\<V> s (Suc b\<^sub>s) (Suc p\<^sub>\<C>) \<leadsto>\<^sub>r S\<^sub>r h b\<^sub>h \<Delta> b\<^sub>\<Delta> (\<V>(b\<^sub>\<V> := y)) (Suc b\<^sub>\<V>) s (Suc b\<^sub>s) p\<^sub>\<C>"
 | ev\<^sub>r_pushcon [simp]: "lookup \<C> p\<^sub>\<C> = Some (PushCon\<^sub>b n) \<Longrightarrow> 
     \<C> \<tturnstile> S\<^sub>r h b\<^sub>h \<Delta> b\<^sub>\<Delta> \<V> b\<^sub>\<V> s (Suc b\<^sub>s) (Suc p\<^sub>\<C>) \<leadsto>\<^sub>r 
       S\<^sub>r (h(b\<^sub>h := (PConst, n), Suc b\<^sub>h := (PConst, 0))) (2 + b\<^sub>h) \<Delta> b\<^sub>\<Delta> (\<V>(b\<^sub>\<V> := b\<^sub>h)) (Suc b\<^sub>\<V>) s 
         (Suc b\<^sub>s) p\<^sub>\<C>"
-| ev\<^sub>r_pushlam [simp]: "lookup \<C> p\<^sub>\<C> = Some (PushLam\<^sub>b p\<^sub>\<C>') \<Longrightarrow> 
+| ev\<^sub>r_pushlam [simp]: "lookup \<C> p\<^sub>\<C> = Some (PushLam\<^sub>b p\<^sub>\<C>' n) \<Longrightarrow> 
     \<C> \<tturnstile> S\<^sub>r h b\<^sub>h \<Delta> b\<^sub>\<Delta> \<V> b\<^sub>\<V> s (Suc b\<^sub>s) (Suc p\<^sub>\<C>) \<leadsto>\<^sub>r 
       S\<^sub>r (h(b\<^sub>h := (PEnv, s b\<^sub>s), Suc b\<^sub>h := (PCode, p\<^sub>\<C>'))) (2 + b\<^sub>h) \<Delta> b\<^sub>\<Delta> (\<V>(b\<^sub>\<V> := b\<^sub>h)) (Suc b\<^sub>\<V>) s 
         (Suc b\<^sub>s) p\<^sub>\<C>"
